@prefix adms: <http://www.w3.org/ns/adms#> .
@prefix rdf: <http://www.w3.org/1999/02/22-rdf-syntax-ns#> .
@prefix epos: <https://www.epos-eu.org/epos-dcat-ap#> .
@prefix dc: <http://purl.org/dc/elements/1.1/> .
@prefix dct: <http://purl.org/dc/terms/> .
@prefix vcard: <http://www.w3.org/2006/vcard/ns#> .
@prefix hydra: <http://www.w3.org/ns/hydra/core#> .
@prefix xsd: <http://www.w3.org/2001/XMLSchema#> .
@prefix schema: <http://schema.org/> .
@prefix dcat: <http://www.w3.org/ns/dcat#> .
@prefix cnt: <http://www.w3.org/2011/content#> .
@prefix locn: <http://www.w3.org/ns/locn#> .
@prefix skos: <http://www.w3.org/2004/02/skos/core#> .
@prefix rdfs: <http://www.w3.org/2000/01/rdf-schema#> .
@prefix http: <http://www.w3.org/2006/http#> .
@prefix owl: <http://www.w3.org/2002/07/owl#> .
@prefix gsp: <http://www.opengis.net/ont/geosparql#> .

<epos:Seismology> a skos:ConceptScheme;
	dct:title "Seismology";
	dct:description "It contains the concepts of Seismology";
.

<epos:Seismologicalproducts> a skos:Concept;
	skos:prefLabel "Seismological products";
	skos:definition "Results of extensive research and technological activies based on the data.";
	skos:inScheme <epos:Seismology>;
	skos:narrower <epos:Historicalearthquakes>, <epos:Macroseismicdata>, <epos:StudiesonEarthquakes>;
.

<epos:Historicalearthquakes> a skos:Concept;
	skos:prefLabel "Historical earthquakes";
	skos:definition "Earthquakes described by a set of numerical parameters such as origin time, epicentre and some description of its effects, most notably magnitude, number of Macroseismic Data Points (MDP) available, and the maximum observed intensity.";
	#skos:inScheme <epos:Seismologicalproducts>;
	skos:broader <epos:Seismologicalproducts>;
	skos:inScheme <epos:Seismology>;
.

<epos:Macroseismicdata> a skos:Concept;
	skos:prefLabel "Macroseismic Data Points";
	skos:definition "The study of any effects of earthquakes that are observable without instruments, such as felt by people, landslides, fissures, knocked-down chimneys, etc. Semi-quantitative expression of the earthquake effects, as derived from written accounts, questionnaires, etc, formalized in terms of macroseismic intensity at a given location. Usually abbreviated as MDP.";
	#skos:inScheme <epos:Seismologicalproducts>; 
	skos:broader <epos:Seismologicalproducts>;
	skos:inScheme <epos:Seismology>;
.

<epos:Studiesonearthquakes> a skos:Concept;
	skos:prefLabel "Studies on earthquakes";
	skos:definition "Published results of scientific investigations.";
	#skos:inScheme <epos:Seismologicalproducts>;
	skos:broader <epos:Seismologicalproducts>;
	skos:inScheme <epos:Seismology>;
.

<PIC:999472675> a schema:Organization;
	schema:identifier [ a schema:PropertyValue;
		schema:propertyID "PIC";
		schema:value "999472675";
	];
	schema:legalName "Istituto Nazionale di Geofisica e Vulcanologia (INGV)"@it;
	schema:address [ a schema:PostalAddress;
		schema:streetAddress "via di Vigna Murata 605";
		schema:addressLocality "Roma";
		schema:postalCode "00143";
		schema:addressCountry "Italy";
	];
	schema:logo "https://data.ingv.it/images/logos/logo_ingv_vertical_two_lines.png"^^xsd:anyURI;
	schema:url "http://www.ingv.it/"^^xsd:anyURI;
	schema:email "ufficiogestionedati@ingv.it";
	schema:telephone "+3906518601";
	schema:contactPoint <PIC:999472675/legalContact>;
	schema:contactPoint <PIC:999472675/financialContact>;
	schema:contactPoint <https://www.epos-eu.org/epos-dcat-ap/Seismology/Facility/AHEAD/scientificContact>;
	schema:contactPoint <https://www.epos-eu.org/epos-dcat-ap/Seismology/Facility/AHEAD/contactPoint>;
	#schema:owns <https://www.epos-eu.org/epos-dcat-ap/Seismology/Facility/AHEAD>;
.

<https://orcid.org/0000-0002-8651-6387> a schema:Person;
	schema:identifier [ a schema:PropertyValue;
		schema:propertyID "orcid";
		schema:value "https://orcid.org/0000-0002-8651-6387";
	];
	schema:familyName "Doglioni";
	schema:givenName "Carlo";
	schema:address [ a schema:PostalAddress;
		schema:streetAddress "Via di Vigna Murata 605";
		schema:addressLocality "Rome";
		schema:postalCode "00143";
		schema:addressCountry "Italy";
	];
	schema:email "segreteria.presidenza@ingv.it";
	schema:telephone "+3906518601";
	schema:url "https://orcid.org/0000-0002-8651-6387"^^xsd:anyURI;
	schema:qualifications "Professor";
	schema:affiliation <PIC:999472675>;
	schema:contactPoint <PIC:999472675/legalContact>;
	schema:contactPoint <PIC:999472675/financialContact>;
.

<http://orcid.org/0000-0001-6147-9981> a schema:Person;
	schema:identifier [ a schema:PropertyValue;
		schema:propertyID "orcid";
		schema:value "http://orcid.org/0000-0001-6147-9981";
	];
	schema:familyName "Rovida";
	schema:givenName "Andrea";
	schema:address [ a schema:PostalAddress;
		schema:streetAddress "via Alfonso Corti 12";
		schema:addressLocality "Milano";
		schema:postalCode "20133";
		schema:addressCountry "ITALY";
	];
	schema:email "andrea.rovida@ingv.it";
	schema:telephone "+390223699257";
	schema:qualifications "Researcher";
	schema:affiliation <PIC:999472675>;
	schema:contactPoint <https://www.epos-eu.org/epos-dcat-ap/Seismology/Facility/AHEAD/scientificContact>;
.

<http://orcid.org/0000-0003-2185-3267> a schema:Person;
	schema:identifier [ a schema:PropertyValue;
		schema:propertyID "orcid";
		schema:value "http://orcid.org/0000-0003-2185-3267";
	];
	schema:familyName "Locati";
	schema:givenName "Mario";
	schema:address [ a schema:PostalAddress;
		schema:streetAddress "via Alfonso Corti 12";
		schema:addressLocality "Milano";
		schema:postalCode "20133";
		schema:addressCountry "ITALY";
	];
	schema:email "mario.locati@ingv.it";
	schema:telephone "+390223699451";
	schema:qualifications "Technologist";
	schema:affiliation <PIC:999472675>;
	schema:contactPoint <https://www.epos-eu.org/epos-dcat-ap/Seismology/Facility/AHEAD/contactPoint>;
.

<PIC:999472675/legalContact> a schema:ContactPoint;
	schema:email "segreteria.presidenza@ingv.it";
	schema:availableLanguage "en";
	schema:contactType "legalContact";
.

<PIC:999472675/financialContact> a schema:ContactPoint;
	schema:email "segreteria.presidenza@ingv.it";
	schema:availableLanguage "en";
	schema:contactType "financialContact";
.

<https://www.epos-eu.org/epos-dcat-ap/Seismology/Facility/AHEAD/scientificContact> a schema:ContactPoint;
	schema:email "andrea.rovida@ingv.it";
	schema:availableLanguage "en";
	schema:contactType "scientificContact";
.

<https://www.epos-eu.org/epos-dcat-ap/Seismology/Facility/AHEAD/contactPoint> a schema:ContactPoint;
	schema:email "mario.locati@ingv.it";
	schema:availableLanguage "en";
	schema:contactType "manager";
.
#
#   -------------------------------- Datasets --------------------------------
#

<https://tsunamiarchive.ingv.it/services/tsunami> a dcat:Dataset;
	dct:title "Historical earthquakes 1000-1899";
	dct:description "Event data (e.g. epicentre, magnitude) for earthquakes archived in AHEAD";
	dct:identifier "https://www.epos-eu.org/epos-dcat-ap/Seismology/Dataset/AHEAD/events";
	adms:identifier [ a adms:Identifier;
		adms:schemeAgency "DDSS-ID";
		skos:notation "WP08-DDSS-024";
	];
	dct:type "http://purl.org/dc/dcmitype/Dataset"^^xsd:anyURI;
	dct:accrualPeriodicity "http://purl.org/cld/freq/irregular"^^xsd:anyURI;
	dct:created "2010-06-01"^^xsd:date;
	dct:modified "2018-09-10"^^xsd:date;
	dct:temporal [ a dct:PeriodOfTime;
		schema:startDate "1000-01-01T00:00:00Z"^^xsd:dateTime;
		schema:endDate "1899-12-31T23:59:59Z"^^xsd:dateTime;
	];
	dct:spatial [ a dct:Location;
		locn:geometry "POLYGON((-34 74,45 74,45 33,-34 33,-34 74))"^^gsp:wktLiteral;
	];
	dcat:theme <epos:Historicalearthquakes>;
	dcat:keyword "event", "earthquake", "seismicity", "catalogue", "magnitude";
	dcat:contactPoint <https://www.epos-eu.org/epos-dcat-ap/Seismology/Facility/AHEAD/scientificContact>;
	dcat:contactPoint <https://www.epos-eu.org/epos-dcat-ap/Seismology/Facility/AHEAD/contactPoint>;
	dct:publisher <PIC:999472675>;
        dcat:distribution <http://www.w3.org/ns/EMTCv2_Full_Dataset>;
.

#
#   -------------------------------- Distributions --------------------------------
#

<http://www.w3.org/ns/EMTCv2_Full_Dataset> a dcat:Distribution ;
	dct:title "EMTC V2 Tsunami Catalogue Full Dataset (OGC WFS)" ;
	dct:description "A unified catalogue containing tsunamis generated in the European and Mediterranean seas since 6150 B.C. to current days. The Catalogue of Euro-Mediterranean Tsunamis (EMTC2.0), realized in ArcGis online, contains 293 tsunamis and is the updated version of EMTC published in 2014.The Italian section of the database was revised in order to implement the new database of tsunami effects along the Italian coasts (ITED). In order to improve the quality of the data, all the Italian tsunamis of seismic origin have been linked to the Parametric Catalogue of Italian Earthquakes (CPTI15) adopted as the reference earthquake catalogue.In the EMTC2.0 two new tsunami events were added, more information enriched the knowledge on the tsunamis present in the Italian section and, accordingly to the new achieved info, some tsunami parameters, such as the reliability, intensity, generating cause, etc. have changed.ITED and EMTCv2 are interconnected and they can be accessed through a purpose-built WebApp that allows the user to easily switch from one database to another. EMTC is interoperable with the database of the Italian Archive of Historical Earthquake Data (ASMI)." ;
	dct:identifier "http://www.w3.org/ns/EMTCv2_Full_Dataset";
	dct:issued "2019-05-02"^^xsd:dateTime;
	dct:modified "2022-07-19"^^xsd:dateTime;
	dct:type "http://publications.europa.eu/resource/authority/distribution-type/WEB_SERVICE"^^xsd:anyURI;
	dct:conformsTo <http://www.w3.org/ns/Tsunami/EMTC_v2>;
	dcat:accessURL <https://www.epos-eu.org/epos-dcat-ap/Seismology/WebService/AHEAD/restful/fdsnws-event/Operation>;
	dct:license "https://creativecommons.org/licenses/by/4.0/"^^xsd:anyURI;
	dct:format "http://publications.europa.eu/resource/authority/file-type/JSON"^^xsd:anyURI;
.


#
#   -------------------------------- Web Services and their documentation --------------------------------
#

<http://www.w3.org/ns/Tsunami/EMTC_v2> a epos:WebService;
	schema:identifier "https://www.epos-eu.org/epos-dcat-ap/Seismology/WebService/AHEAD/restful/fdsnws-event";
	schema:description "FDSN-event web service providing event parameters for historical earthquakes from AHEAD, the European Archive of Historical Earthquake Data";
	dcat:theme <epos:Historicalearthquakes>;
	schema:name "Historical earthquakes 1000-1899 (FDSN-event)";
	hydra:entrypoint "https://www.emidius.eu/fdsnws/event/1/application.wadl"^^xsd:anyURI;
	schema:provider <PIC:999472675>;
	schema:datePublished "2012-12-01"^^xsd:date;
	schema:dateModified "2018-09-10"^^xsd:date;
	dct:spatial [ a dct:Location;
		locn:geometry "POLYGON((-33.5 73.5,34.0 73.5,34.0 33.5,-33.5 33.5,-33.5 73.5))"^^gsp:wktLiteral;
	];
	hydra:supportedOperation <https://www.epos-eu.org/epos-dcat-ap/Seismology/WebService/AHEAD/restful/fdsnws-event/Operation>;
	schema:keywords "seismology", "seismicity", "catalogue", "earthquake", "magnitude", "seismic hazard", "historical";
	dct:license "https://www.emidius.eu/AHEAD/description.php#copyright"^^xsd:anyURI;
	dct:temporal [ a dct:PeriodOfTime;
		schema:startDate "1000-01-01T00:00:00Z"^^xsd:dateTime;
		schema:endDate "1899-12-31T23:59:59Z"^^xsd:dateTime;
	];
	dcat:contactPoint <https://www.epos-eu.org/epos-dcat-ap/Seismology/Facility/AHEAD/contactPoint>;
	dcat:contactPoint <https://www.epos-eu.org/epos-dcat-ap/Seismology/Facility/AHEAD/scientificContact>;
	dct:conformsTo <https://www.epos-eu.org/epos-dcat-ap/Seismology/WebService/AHEAD/APIDocumentation/fdsnws-event>;
.

<https://www.epos-eu.org/epos-dcat-ap/Seismology/WebService/AHEAD/APIDocumentation/fdsnws-event> a hydra:ApiDocumentation;
      	hydra:title "ahead-fdsnws-event documentation" ;
      	hydra:description "Documentation for the fdsnws-event webservice" ;
      	hydra:entrypoint "https://www.emidius.eu/AHEAD/services/events.php"^^xsd:anyURI ;
.


#
#   -------------------------------- Operations --------------------------------
#

<https://www.epos-eu.org/epos-dcat-ap/Seismology/WebService/AHEAD/restful/fdsnws-event/Operation> a hydra:Operation;
	hydra:method "GET"^^xsd:string;
	hydra:returns "application/xml";
	hydra:property[ a hydra:IriTemplate;
		hydra:template "https://www.emidius.eu/fdsnws/event/1/query{?starttime, endtime, eventid, minlatitude, maxlatitude, minlongitude, maxlongitude, latitude, longitude, minradius, maxradius, minradiuskm, maxradiuskm, minmagnitude, maxmagnitude, contributor, contributorid, format, orderby, includeallorigins, includeallmagnitudes, updatedafter, limit, nodata}"^^xsd:string;
			hydra:mapping[ a hydra:IriTemplateMapping;
				hydra:variable "starttime"^^xsd:string;
				hydra:property "schema:startDate";
				schema:valuePattern "YYYY-MM-DDThh:mm:ss";
				rdfs:range "xsd:dateTime";
				rdfs:label "Start time"@en;
				schema:minValue "1000-01-01T00:00:00";
				schema:maxValue "1899-12-31T23:59:59";
				schema:defaultValue "1000-01-01T00:00:00";
				hydra:required "true"^^xsd:boolean;
			];
			hydra:mapping[ a hydra:IriTemplateMapping;
				hydra:variable "endtime"^^xsd:string;
				hydra:property "schema:endDate";
				schema:valuePattern "YYYY-MM-DDThh:mm:ss";
				rdfs:range "xsd:dateTime";
				rdfs:label "End time"@en;
				schema:minValue "1000-01-01T00:00:00";
				schema:maxValue "1899-12-31T23:59:59";
				schema:defaultValue "1899-12-31T23:59:59";
				hydra:required "true"^^xsd:boolean;
			];
			hydra:mapping[ a hydra:IriTemplateMapping;
				hydra:variable "eventid"^^xsd:string;
				rdfs:range "xsd:string";
				rdfs:label "Event ID"@en;
				hydra:required "false"^^xsd:boolean;
			];
			hydra:mapping[ a hydra:IriTemplateMapping;
				hydra:variable "minlatitude"^^xsd:string;
				hydra:property "epos:southernmostLatitude";
				rdfs:range "xsd:float";
				rdfs:label "Minimum latitude"@en;
				schema:minValue "33.0000";
				schema:maxValue "74.0000";
				schema:defaultValue "33.0000";
				hydra:required "false"^^xsd:boolean;
			];
			hydra:mapping[ a hydra:IriTemplateMapping;
				hydra:variable "maxlatitude"^^xsd:string;
				hydra:property "epos:northernmostLatitude";
				rdfs:range "xsd:float";
				rdfs:label "Maximum latitude"@en;
				schema:minValue "33.0000";
				schema:maxValue "74.0000";
				schema:defaultValue "74.0000";
				hydra:required "false"^^xsd:boolean;
			];
			hydra:mapping[ a hydra:IriTemplateMapping;
				hydra:variable "minlongitude"^^xsd:string;
				hydra:property "epos:westernmostLongitude";
				rdfs:range "xsd:float";
				rdfs:label "Minimum longitude"@en;
				schema:minValue "-34.0000";
				schema:maxValue "34.0000";
				schema:defaultValue "-34.0000";
				hydra:required "false"^^xsd:boolean;
			];
			hydra:mapping[ a hydra:IriTemplateMapping;
				hydra:variable "maxlongitude"^^xsd:string;
				hydra:property "epos:easternmostLongitude";
				rdfs:range "xsd:float";
				rdfs:label "Maximum longitude"@en;
				schema:minValue "-34.0000";
				schema:maxValue "34.0000";
				schema:defaultValue "34.0000";
				hydra:required "false"^^xsd:boolean;
			];
			hydra:mapping[ a hydra:IriTemplateMapping;
				hydra:variable "latitude"^^xsd:string;
				rdfs:range "xsd:float";
				rdfs:label "Center latitude"@en;
				schema:minValue "33.0000";
				schema:maxValue "74.0000";
				hydra:required "false"^^xsd:boolean;
			];
			hydra:mapping[ a hydra:IriTemplateMapping;
				hydra:variable "longitude"^^xsd:string;
				rdfs:range "xsd:float";
				rdfs:label "Center longitude"@en;
				schema:minValue "-34.0000";
				schema:maxValue "34.0000";
				hydra:required "false"^^xsd:boolean;
			];
			hydra:mapping[ a hydra:IriTemplateMapping;
				hydra:variable "minradius"^^xsd:string;
				rdfs:range "xsd:float";
				rdfs:label "Minimum search radius (degrees)"@en;
				schema:minValue "0.00";
				schema:maxValue "5.00";
				hydra:required "false"^^xsd:boolean;
			];
			hydra:mapping[ a hydra:IriTemplateMapping;
				hydra:variable "maxradius"^^xsd:string;
				rdfs:range "xsd:float";
				rdfs:label "Maximum search radius (degrees)"@en;
				schema:minValue "0.00";
				schema:maxValue "5.00";
				hydra:required "false"^^xsd:boolean;
			];
			hydra:mapping[ a hydra:IriTemplateMapping;
				hydra:variable "minradiuskm"^^xsd:string;
				rdfs:range "xsd:float";
				rdfs:label "Minimum search radius (in km)"@en;
				schema:minValue "0.00";
				schema:maxValue "500.00";
				hydra:required "false"^^xsd:boolean;
			];
			hydra:mapping[ a hydra:IriTemplateMapping;
				hydra:variable "maxradiuskm"^^xsd:string;
				rdfs:range "xsd:float";
				rdfs:label "Maximum search radius (in km)"@en;
				schema:minValue "0.00";
				schema:maxValue "500.00";
				hydra:required "false"^^xsd:boolean;
			];
			hydra:mapping[ a hydra:IriTemplateMapping;
				hydra:variable "minmagnitude"^^xsd:string;
				rdfs:range "xsd:float";
				rdfs:label "Minimum magnitude (Mw)"@en;
				schema:minValue "0.0";
				schema:maxValue "10.0";
				hydra:required "false"^^xsd:boolean;
			];
			hydra:mapping[ a hydra:IriTemplateMapping;
				hydra:variable "maxmagnitude"^^xsd:string;
				rdfs:range "xsd:float";
				rdfs:label "Maximum magnitude (Mw)"@en;
				schema:minValue "0.0";
				schema:maxValue "10.0";
				hydra:required "false"^^xsd:boolean;
			];
			hydra:mapping[ a hydra:IriTemplateMapping;
				hydra:variable "contributor"^^xsd:string;
				rdfs:range "xsd:string";
				rdfs:label "Data contributor code"@en;
				hydra:required "false"^^xsd:boolean;
			];
			hydra:mapping[ a hydra:IriTemplateMapping;
				hydra:variable "contributorid"^^xsd:string;
				rdfs:range "xsd:string";
				rdfs:label "Contributor event ID"@en;
				hydra:required "false"^^xsd:boolean;
			];
			hydra:mapping[ a hydra:IriTemplateMapping;
				hydra:variable "format"^^xsd:string;
				rdfs:range "xsd:string";
				rdfs:label "Output format"@en;
				hydra:property "schema:encodingFormat";
				http:paramValue "xml";
				http:paramValue "text";
				http:paramValue "json";
				schema:defaultValue "xml";
				hydra:required "false"^^xsd:boolean;
			];
			hydra:mapping[ a hydra:IriTemplateMapping;
				hydra:variable "orderby"^^xsd:string;
				rdfs:range "xsd:string";
				rdfs:label "Output ordering"@en;
				http:paramValue "time";
				http:paramValue "time-asc";
				http:paramValue "magnitude";
				http:paramValue "magnitude-asc";
				schema:defaultValue "time";
				hydra:required "false"^^xsd:boolean;
			];
			hydra:mapping[ a hydra:IriTemplateMapping;
				hydra:variable "includeallorigins"^^xsd:string;
				rdfs:range "xsd:boolean";
				rdfs:label "Include all origins"@en;
				schema:defaultValue "false";
				http:paramValue "true";
				http:paramValue "false";
				hydra:required "false"^^xsd:boolean;
			];
			hydra:mapping[ a hydra:IriTemplateMapping;
				hydra:variable "includeallmagnitudes"^^xsd:string;
				rdfs:range "xsd:boolean";
				rdfs:label "Include all magnitudes"@en;
				schema:defaultValue "false";
				http:paramValue "true";
				http:paramValue "false";
				hydra:required "false"^^xsd:boolean;
			];
			hydra:mapping[ a hydra:IriTemplateMapping;
				hydra:variable "limit"^^xsd:string;
				rdfs:range "xsd:integer";
				rdfs:label "Limit the no. of output entries"@en;
				schema:minValue "1";
				schema:maxValue "5000";
				schema:defaultValue "300";
				hydra:required "true"^^xsd:boolean;
			];
			hydra:mapping[ a hydra:IriTemplateMapping;
				hydra:variable "updatedafter"^^xsd:string;
				rdfs:range "xsd:dateTime";
				rdfs:label "Update after"@en;
				schema:minValue "2010-01-01T00:00:00";
				hydra:required "false"^^xsd:boolean;
			];
			hydra:mapping[ a hydra:IriTemplateMapping;
				hydra:variable "nodata"^^xsd:string;
				rdfs:range "xsd:string";
				rdfs:label "Status code for "@en;
				http:paramValue "204";
				http:paramValue "404";
				schema:defaultValue "204";
				hydra:required "false"^^xsd:boolean;
			];
	];
.


